Port Poly1305_32 to fstar master / kremlin fstar-master

code/poly1305_32/Hacl.Test.Poly1305_32.fst
@@ -8,7 +8,7 @@ open FStar.Buffer
 open Hacl.Cast
 open Hacl.Poly1305_32
 
-val main: unit -> ST FStar.Int32.t
+val main: unit -> ST C.exit_code
   (requires (fun h -> True))
   (ensures  (fun h0 r h1 -> True))
 let main () =
@@ -36,6 +36,6 @@ let main () =
     0x4auy; 0xbfuy; 0xf6uy; 0xafuy; 0x41uy; 0x49uy; 0xf5uy; 0x1buy
     ] in
   crypto_onetimeauth mac plaintext len' key;
-  TestLib.compare_and_print (C.string_of_literal "Poly1305-32bits") expected mac macsize;
+  TestLib.compare_and_print (C.String.of_literal "Poly1305-32bits") expected mac macsize;
   pop_frame();
-  C.exit_success
+  C.EXIT_SUCCESS
